Added some more code

Elgamal/src/Elgamal.lean
@@ -1,48 +1,185 @@
 import data.fintype data.nat.basic
+       data.zmod.basic algebra.group_power
+
+
+namespace Zeroknowledgeproof
+variables (p : ℕ) (q : ℕ) (r : ℕ+)
+  (Hp : nat.prime p)
+  (Hq : nat.prime q)
+  (Hdiv : p = q * r + 1)
+  (g : zmodp p Hp) /- g is a generator -/
+  (Hg : g^q = 1)   /- of order q -/
+  (w : zmodp q Hq) /- private key-/
+  (h : zmodp p Hp)
+  (Hh : h = g^w.val)
+
+/- 
+A Schnorr group is a large prime-order subgroup of ℤ∗𝑝, 
+the multiplicative group of integers modulo 𝑝. 
+To generate such a group, we find 𝑝=𝑞𝑟+1 such that 𝑝 and 𝑞
+are prime.Then, we choose any ℎ
+in the range 1<ℎ<𝑝 such that ℎ^r ≠ 1 (mod𝑝)
+The value 𝑔=ℎ^𝑟(mod𝑝) is a generator of a subgroup ℤ∗𝑝 of order 𝑞.
+By Fermat's little theorem
+g^q = h^(rq) = h^(p-1) = 1 (mod p)
+
+-/
+
+def elgamal_enc (m : zmodp p Hp) (r : zmodp q Hq) :=
+  (g^r.val, g^m.val * h^r.val)
+
+def elgamal_dec (c : zmodp p Hp × zmodp p Hp) :=
+     c.2 * (c.1^w.val)⁻¹ 
+    
+def multiply_cipher (c₁ c₂ : zmodp p Hp × zmodp p Hp) :=
+  (c₁.1 * c₂.1, c₁.2 * c₂.2)
+
+
+#check elgamal_enc p q Hp Hq g h 
+#check elgamal_dec p q Hp Hq w 
+#check multiply_cipher p Hp
+
+lemma prime5: nat.prime 5 := 
+begin 
+ unfold nat.prime,
+ split, sorry, 
+ intros m Hm, sorry 
+end 
+/- It's pretty fase -/
+#eval (13^1990 : zmodp 5 prime5)
+
+include Hh
+lemma elgama_enc_dec_identity :  
+ ∀ m r, elgamal_dec p q Hp Hq w (elgamal_enc p q Hp Hq g h m r) 
+        = g^m.val :=
+begin
+ intros m r, 
+ unfold elgamal_enc elgamal_dec,
+ simp, rw Hh, sorry 
+end 
+         
+end Zeroknowledgeproof
+
+namespace Interactive 
+
+variables (p : ℕ) (Hp : nat.prime p)
+          (g : zmodp p Hp)
+
+/- 
+universes u v
+inductive communication : zmodp p Hp -> Type u
+| commitment : ∀ k, communication k
+| challenge : ∀ k, communication k
+| response : ∀ k, communication k
+
+open communication
+/- Both parties are honest. zero knowledge proof -/
+inductive zeroknowledge : ∀ (t : zmodp p Hp), communication p Hp t → Type u
+| first_step : ∀ (r k : zmodp p Hp), k = g^r.val → zeroknowledge k (commitment k)
+| second_step : ∀ (k c : zmodp p Hp), zeroknowledge k (commitment k) → 
+    zeroknowledge c (challenge c)
+| final_step : ∀ (s k c a : zmodp p Hp), s = k + c * a → 
+          zeroknowledge c (challenge c) → zeroknowledge s (response s)
+    
+-/
+/- I claim that this always checks out -/
+
+universes u v
+inductive communication : Type u
+| commitment : ∀ (k : zmodp p Hp), communication
+| challenge  : ∀ (k c : zmodp p Hp), communication
+| response   : ∀ (k c s : zmodp p Hp), communication
+
+/- /- zero knowledge proof of zkp {x | g^x = h} -/  -/
+open communication
+inductive zeroknowledge (x h : zmodp p Hp) (Hf : h = g^x.val) : 
+    communication p Hp → Type u
+| first_step (r k : zmodp p Hp) : k = g^r.val → zeroknowledge (commitment k)
+| second_step (k c : zmodp p Hp) : zeroknowledge (commitment k) → 
+    zeroknowledge (challenge k c)
+| final_step (r k c s : zmodp p Hp) : s = r + c * x →
+      /- How to connect r and k ? k = g^r.val or this can be 
+      inferred from zeroknowledge (challenge k c). What if 
+      prover try to cheat -/
+          zeroknowledge (challenge k c) → zeroknowledge (response k c s)
+
+axiom unique_element_in_zmodp : ∀ (k : zmodp p Hp), ∃ r : zmodp p Hp, k = g^r.val
+
+axiom discrete_log : ∀ (k r₁ r₂ : zmodp p Hp), k = g^r₁.val -> k = g^r₂.val -> 
+           r₁ = r₂  
+
+open zeroknowledge
+#check zeroknowledge
+lemma first_constructor :  ∀ (k x h : zmodp p Hp) (Hf : h = g^x.val), 
+  zeroknowledge p Hp g x h Hf (commitment k) :=
+  begin 
+    intros, have h := unique_element_in_zmodp p Hp g k, 
+    sorry,
+  end
+
  
+lemma proof_of_correctness : ∀ (x h : zmodp p Hp) (Hf : h = g^x.val) 
+    (k c s : zmodp p Hp), 
+    zeroknowledge p Hp g x h Hf (response k c s) → 
+    g^s.val = k * h^c.val :=
+    begin 
+    intros x h Hf k c s Hzkp, 
+    destruct Hzkp, 
+    {intros r k Ha Hr, injection Hr},
+    {intros k c a Hr, injection Hr},
+    intros r k c s Hs Ha Hr Hzero, clear Hr, 
+    destruct Ha, 
+    intros _ _ _ Hr₁, injection Hr₁, 
+    intros k₁ c₁ Hc Hr₁ Ha₁, injection Hr₁, 
+    destruct Hc, intros, 
+    
+    end 
+
+lemma proof_of_knowlege : 
+
 namespace Elgamal
 
 /- define a group on finite type -/
 universe u
 variables (A : Type u) (Hf : fintype A)
-(gOp : A -> A -> A) (e : A) (inv : A -> A)
+(gop : A -> A -> A) (e : A) (inv : A -> A)
 
 class group  :=
-  (associativity : ∀ x y z : A, gOp x (gOp y z) = 
-                                gOp (gOp x y) z)
-  (left_identity : ∀ x : A, gOp e x = x)
-  (right_identity : ∀ x : A, gOp x e = x)
-  (left_inverse : ∀ x : A, gOp (inv x) x = e)
-  (right_inverse : ∀ x : A, gOp x (inv x) = e)
+  (associativity : ∀ x y z : A, gop x (gop y z) = 
+                                gop (gop x y) z)
+  (left_identity : ∀ x : A, gop e x = x)
+  (right_identity : ∀ x : A, gop x e = x)
+  (left_inverse : ∀ x : A, gop (inv x) x = e)
+  (right_inverse : ∀ x : A, gop x (inv x) = e)
  
 
 def group_pow (x : A) : ℕ → A 
 | 0 := e
-| (n + 1) := gOp x (group_pow n)
+| (n + 1) := gop x (group_pow n)
 
-variable Hg : group A gOp e inv
-include Hg 
+variable (G : group A gop e inv)
+include G 
 
 lemma group_exp_identity :
- ∀ (n : ℕ), group_pow A gOp e e n = e :=
+ ∀ (n : ℕ), group_pow A gop e e n = e :=
   begin
   intro n, induction n,
   /- simplification would do the job -/
   /- simplify it and rewrite in Ih, follwed right_identity -/
   {simp [group_pow]},
   {dsimp [group_pow], 
-   rewrite n_ih, apply (group.left_identity gOp e inv e)}
+   rewrite n_ih, apply (group.left_identity gop e inv e)}
   end
 
 lemma group_exp_plus : ∀ (n m : ℕ) (x : A), 
-  group_pow A gOp e x (n + m) = 
-  gOp (group_pow A gOp e x n) (group_pow A gOp e x m) := 
+  group_pow A gop e x (n + m) = 
+  gop (group_pow A gop e x n) (group_pow A gop e x m) := 
   begin 
   intros n, 
   induction n, 
   {intros m x, simp [group_pow],
    rewrite
-   group.left_identity gOp e inv (group_pow A gOp e x m)},
+   group.left_identity gop e inv (group_pow A gOp e x m)},
   {intros m x,
    simp [group_pow],
    rewrite nat.add_succ,
@@ -50,9 +187,21 @@ lemma group_exp_plus : ∀ (n m : ℕ) (x : A),
    rewrite <- (group.associativity gOp e inv x)}
   end
 
-  
-              
+  lemma group_exp_mult : ∀ (n m : ℕ) (x : A), 
+  group_pow A gop e x (n * m) = 
+  group_pow A gop e (group_pow A gop e x n) m := 
+  begin 
+   intros n, induction n,
+   sorry,
+   sorry
+  end
 
+class abelian_group := 
+  (commutative : ∀ x y, gop x y = gop y x)
+
+  #check (abelian_group A gop e inv G)
+
+class cyclic_group (g : A) (order : ℕ+) 
 
 end Elgamal
 
